src/opt/MemInv.v
@@ -1,0 +1,120 @@
+Require Import Basics.
+Require Import Bool.
+Require Import List.
+
+Require Import sflib.
+Require Import paco.
+Require Import respectful5.
+
+Require Import Axioms.
+Require Import Basic.
+Require Import Event.
+Require Import Time.
+Require Import Language.
+Require Import Memory.
+Require Import Thread.
+Require Import Configuration.
+Require Import Simulation.
+
+Set Implicit Arguments.
+
+Module MemInv.
+  Definition t := Memory.t.
+
+  Inductive sem (inv:t): forall (local_src local_tgt:Memory.t), Prop :=
+  | sem_intro
+      local_tgt
+      (DISJOINT: Memory.disjoint local_tgt inv):
+      sem inv (Memory.join local_tgt inv) local_tgt
+  .
+
+  Lemma add
+        inv
+        local1_src global1_src
+        local1_tgt global1_tgt local2_tgt global2_tgt
+        (LE1_SRC: Memory.le local1_src global1_src)
+        (LE1_TGT: Memory.le local1_tgt global1_tgt)
+        (SIM1: sim_memory global1_src global1_tgt)
+        (INV1: sem inv local1_src local1_tgt)
+        (ADD_TGT: Memory.add local1_tgt global1_tgt local2_tgt global2_tgt):
+    exists local2_src global2_src,
+      <<LE1_SRC: Memory.le local2_src global2_src>> /\
+      <<SIM2: sim_memory global2_src global2_tgt>> /\
+      <<INV2: sem inv local2_src local2_tgt>> /\
+      <<ADD_SRC: Memory.add local1_src global1_src local2_src global2_src>>.
+  Proof.
+    inv SIM1. inv INV1. inv ADD_TGT.
+    memtac. subst ohs. memtac.
+    rewrite <- Memory.join_assoc in SPLITS.
+    apply Memory.splits_join_inv in SPLITS; memtac.
+    exploit Memory.join2_splits; try apply JOINC; memtac.
+    { splits; memtac. }
+    { eapply Memory.splits_disjoint; [|eauto].
+      symmetry. eapply Memory.splits_disjoint; [|eauto].
+      memtac.
+    }
+    i. des. subst.
+    exists (Memory.join local2_tgt inv).
+    exists (Memory.join (Memory.join local2_tgt (Memory.join inv ohs0)) addendum).
+    splits.
+    - rewrite Memory.join_assoc, <- Memory.join_assoc.
+      econs; eauto. repeat (splits; memtac).
+      symmetry in ADDENDUM0. eapply Memory.splits_disjoint in ADDENDUM0; eauto.
+      memtac.
+    - econs. apply Memory.splits_join.
+      + memtac. splits; memtac.
+      + apply Memory.splits_join; eauto.
+        * memtac.
+        * reflexivity.
+      + reflexivity.
+    - econs. memtac.
+    - rewrite -> Memory.join_assoc. econs; memtac.
+      + apply Memory.splits_join; memtac.
+      + symmetry in ADDENDUM0. eapply Memory.splits_disjoint in ADDENDUM0; eauto.
+        memtac. splits; memtac.
+  Qed.
+
+  Lemma remove_tgt
+        inv local1_src local1_tgt local2_tgt
+        loc from to msg
+        (INV: sem inv local1_src local1_tgt)
+        (REMOVE: Memory.remove loc from to msg local1_tgt local2_tgt):
+    exists (LT: Time.lt from to),
+      <<DISJOINT: Memory.disjoint inv (Memory.singleton loc msg LT)>> /\
+      <<INV: sem (Memory.join inv (Memory.singleton loc msg LT)) local1_src local2_tgt>>.
+  Proof.
+    inv INV. memtac.
+    exists LT. splits; memtac.
+    rewrite <- Memory.join_assoc, Memory.join_comm.
+    econs. memtac. splits; memtac.
+  Qed.
+
+  Lemma remove_src
+        inv1 inv2 local1_src local1_tgt
+        loc from to msg
+        (INV: sem inv1 local1_src local1_tgt)
+        (REMOVE: Memory.remove loc from to msg inv1 inv2):
+    exists (LT: Time.lt from to) local2_src,
+      <<REMOVE: Memory.remove loc from to msg local1_src local2_src>> /\
+      <<INV: sem inv2 local2_src local1_tgt>>.
+  Proof.
+    inv INV. memtac.
+    exists LT. eexists. splits; memtac.
+    rewrite Memory.join_assoc. econs; memtac. splits; memtac.
+  Qed.
+
+  Lemma sem_bot local:
+    sem Memory.bot local local.
+  Proof.
+    rewrite <- (Memory.bot_join local) at 1.
+    econs. memtac.
+  Qed.
+
+  Lemma sem_bot_inv
+        local_src local_tgt
+        (SEM: sem Memory.bot local_src local_tgt):
+    local_src = local_tgt.
+  Proof.
+    inv SEM. apply Memory.bot_join.
+  Qed.
+End MemInv.
